\section{Endogenous growth}\label{learning-by-doing}
\subsubsection{Introduction}
In the previous models we assumed that technical progress, which is one of the main factors of growth were exogenous. This does not sufficiently explain economic growth as a result of innovation and technical progress. 

\subsubsection{General assumptions}
\begin{enumerate}
    \item Experience creates more efficient ways of producing with the same amount of input
    \item New knowledge is a by-product of capital investment into machines
        \begin{itemize}
            \item Workers can learn how to be more efficient with new equipment
            \item Investment in capital units such as machines drives increase in technical progress through the learning by doing process
        \end{itemize}
    \item Knowledge is a pure public good i.e. non-rival and non-excludable. In other words, once knowledge and experience is found one cannot prohibit others from using the same knowledge. 
    \item Perfect Competition, identical firms. 
\end{enumerate}

\subsubsection{The firms}

\begin{equation}
    A(t)=\Lambda \Big[ K(t), L(t) \Big]
\end{equation}

\begin{equation*}
    Y_i = F(K_i, AL_i)
\end{equation*}

\begin{equation*}
   y_i = AL_i \cdot f(k_i)
\end{equation*}

\begin{equation*}
    \pi_i = AL_i \cdot f(k_i) - RK_i - WL_i \\
    \implies \Pi_i = AL_i \cdot f(k_i) - RK_i - WL_i = 
\end{equation*}

\begin{equation*}
    \frac{\partial \pi_i}{L_i} = A \cdot f(k_i) - R \cdot k_i \cdot A - W = 0
\end{equation*}

\begin{equation*}
    \frac{\partial \pi_i}{k_i} = A \cdot Li \cdot f'(k) -  R \cdot L_i \cdot A = 0 \implies f'(k_i) = R 
\end{equation*}

\begin{equation*}
    W=A \bigg[ f(k_{i})-k_{i}f'(k_{i}) \bigg]
\end{equation*}

\begin{equation*}
    Y=\sum_{i=1}^{e}=eF(K_{i},AL_{i})=F\bigg[ ek_{i}, A(eL_{i})\bigg]=F(K,AL)
\end{equation*}

\begin{equation*}
\begin{aligned}
    y=\frac{Y}{AL}=f(k) && \text{Where, }  k=k_{i}
\end{aligned}
\end{equation*}

\begin{equation*}
    R=\frac{\partial F}{\partial K}(K_{i},AL_{i})=\frac{\partial F}{\partial K}\bigg( (eK;A(eL)\bigg)=\frac{\partial F}{\partial K}(K;AL)=f'(k)
\end{equation*}



\begin{equation}
    \dot { K } = Y - C = a k - Z ( t )
\end{equation}

\begin{align}
   a - \bar{g}_c > 0
&&
\beta = 0 
\end{align}


\input{1_0_Growth_Theory/1_5_1_AK_Model.tex}

