\subsection{Learning by Doing}

\begin{align*}
    A=B(\cdot)K^{\phi} && B>0 && \phi>0
\end{align*}

\begin{align*}
    aK \to \phi=1 && B(L_{0})=\frac{a^{\frac{1}{1-\alpha}}}{L_{0}} && n=0
\end{align*}

\subsubsection{Solow Version}

\begin{equation*}
    Y=K^\alpha(AL)^{1-\alpha}=K^{\alpha}(B\cdot K^{\phi}\cdot L)^{1-\alpha}
\end{equation*}
\begin{equation*}
    Y=K^{\alpha+\phi(1-\alpha)}(BL)^{1-\alpha}   
\end{equation*}
 
Define $\Psi$, as $\Psi=\alpha+\phi(1-\alpha)$. 
 
\begin{equation*}
    S=sY=s\cdot K^\Psi\cdot(BL)^{1-\alpha}
\end{equation*}

As previously, $\Dot{K}=S$; 

\begin{equation*}
    g_{K}=\frac{\Dot{K}}{K}=s\cdot K^{\Psi-1}(BL)^{1-\alpha}
\end{equation*}

\begin{equation*}
    \frac{\Dot{g}_{K}}{g_{K}}=(\Psi-1)g_{K}+(1-\alpha)n
\end{equation*}

\begin{equation*}
    \Dot{g}_{K}=(Psi-1)g_{K}^2+/(1-\alpha)\cdot n \cdot g_{k}
\end{equation*}
\begin{equation*}
    \Dot{g}_{K}=(1-\alpha)\cdot n \cdot g_{K}-(1-\Psi)g_{K}^2
\end{equation*}

\begin{equation*}
    \Dot{g}_{k}=0 \implies g_{k} \text{is constant}
\end{equation*}

\begin{equation*}
    g_{k}^*=\frac{(1-\alpha)n}{1-\Psi}
\end{equation*}

If the steady state equilibrium is stable: 
\begin{equation*}
    \frac{\partial \Dot{g}_{k}}{\partial g_{K}}<0 \implies(1-\alpha)n-2(1-\Psi)g_{k}^*<0 \implies (1-\alpha)n-2(1-\Psi)\frac{(1-\alpha)n}{1-\Psi}<0 \implies 
    -(1-\alpha)n<0 
\end{equation*}


Implying that equilibrium is only stable iff the population is growing. 

\begin{equation*}
    g_{K}^*>0 \implies 1-\Psi>0 \implies \Psi<1
\end{equation*}


\input{1_0_Growth_Theory/1_5_3_Romer_1990.tex}
