\section{A prototype model: simulation and empirical validation}


\subsection{Uncertainty}

\begin{equation*}
\begin{aligned}
    \underset{C_t, L_t}{\text{max}}   E_t \Bigg\{ \sum^{\infty}_{t = \tau} \left( 1 + \rho \right)^{- (t - \tau} \cdot \left[  \frac{C_t^{1 - \theta} -1}{1 - \theta} + b \frac{(1 - L_t)^{1 - \chi} - 1}{1 - \chi} \right] \Bigg\} \\
   \text{subject to} && W_tL_t + R_tK_t - C_t - \delta K_t - T_t
\end{aligned}
\end{equation*}

Instead of maximizing utility as we did in the cases with perfect information, we now have to maximize Expected Utility $E_t$.



We need to set up a Current Value Hamiltonian (CVH), which will be:

$$
H_t = E_t \Bigg\{ \sum^{\infty}_{t = \tau} \left( 1 + \rho \right)^{- (t - \tau} \cdot \left[  \frac{C_t^{1 - \theta} -1}{1 - \theta} + b \frac{(1 - L_t)^{1 - \chi} - 1}{1 - \chi} \right] \Bigg\} + \lambda_t \left( W_tL_t + R_tK_t - C_t - \delta K_t - T_t \right)
$$

Deriving the first order conditions to solve this problem:

\begin{enumerate}[(1)]
    \item $$\frac{\partial H}{\partial C_t} \equiv \frac{\partial H}{\partial C_t} E_t \frac{C_t^{1 - \theta} - 1}{1 - \theta} - \frac{\partial H}{\partial C_t} E_t \lambda_t C_t = 0 \implies E_t C_t^{- \theta} = E_t \lambda_t $$
    
    \item $$\frac{\partial H}{\partial L_t} -b \left( 1 - L_t \right)^{ - \chi} + \lambda_t W_t = 0$$
    
        \item $$\frac{\partial H}{\partial K_t} E_t \lambda_t \cdot ( R_t - \delta ) = - E_t (\lambda_t - \lambda_{t - 1}) + \rho \lambda_{t - 1} $$

\end{enumerate}


$$
E_t \lambda_{t+1} \cdot \mathcal{R}_{t+1} = - E_t \lambda_{t+1} + (1 + \rho) \lambda_t
$$

$$
E_t (1 + \mathcal{R}_{t+1}) \lambda_{t +1} = ( 1 + \rho) \lambda_{t}
$$


$$
E_t \lambda_{t +1}^{- \theta} \cdot (1 + \mathcal{R}_{t +1}) = (1 + \rho ) \cdot C_t^{- \theta}
$$


$$
C_t^{- \theta} = \frac{1}{1 + \rho} \cdot E_t C_{t + 1}^{- \theta} \cdot (1 + \mathcal{R}_{t +1})
$$
Required assumption: Probability Distribution is stable. Why?
Correct??



\subsection{An exact solution to an approximate problem}
\paragraph{Log-Linerization of the model}
$$
X_{t+1} = f (X_t) \cdot e^{u_t}
$$

$$
\ln X_{t+1} = \ln f(X_t) + U_t
$$

$$
\ell_{t+1}
$$

$$
\Tilde{X}_{t} = \frac{X_t - X^*}{X^*} \implies \frac{X_t}{X^*} = 1 + \Tilde{X}_{t}
$$

$$
\ln \left( \frac{X_t}{X^*} \right) =  \Tilde{X}_{t}
$$

$$
\Tilde{X}_{t} = \ln X_t - \ln X^*
$$

$$
\frac{dX_t}{X^*} = d\ln X_t = \frac{(X_t^* dX_{t}) - X^*}{X^*}
$$

$$
\frac{dX_t}{X^*} \approx  \ln \left( \frac{X_t}{X^*} \right)
$$

$$
(8) \Tilde{A} = 
$$

Consumption Euler Equation on log-linear form:
$$
- \theta C^{* - \theta} \cdot \frac{\partial C_t}{C^*} = \frac{1}{1 + \rho} \left[ (1 + R)^* \cdot (- \theta) C^{* - \theta} \cdot \frac{d E_t C_{t+1}}{C^*} + C^{* - \theta} \cdot d E_t R_{t+1}   \right]
$$

Where $\frac{\partial C_t}{C^*}$ is $\Tilde{C}_t$ and $\frac{d E_t C_{t+1}}{C^*}$ is $E_t\Tilde{C}_{t+1}$

By cancelling terms and substituting our new variables we get:

\begin{equation}
- \theta \Tilde{C}_t = \frac{1}{1 + \rho} \left[ (1 + R)^* \cdot (- \theta) C^{* - \theta} \cdot E_t\Tilde{C}_{t+1} + R^*  \frac{d E_t R_{t+1}}{R^*}   \right]
\end{equation}

$R^* = \rho$

In this equation $\frac{d E_t R_{t+1}}{R^*}$ can be written as $E_t \Tilde{R}_{t+1}$

\begin{equation}\tag{$\Tilde{1}$}
    E_t\Tilde{C}_{t+1} - \Tilde{C}_t = e_1 E_t \Tilde{R}_{t + 1}
    \end{equation}
    
    $$
    e_1 = \frac{\rho}{\theta (1 + \rho )} > 0
    $$


\begin{equation}\tag{(3)}
W_t = (1 - \alpha) A_t^{1 - \alpha} \cdot \left( \frac{K_t}{L_t}  \right)^{\alpha} 
\end{equation}

\begin{equation}\tag{$\Tilde{3}$}
\Tilde{W}_t = (1 - \alpha) \Tilde{A}_t + \left( \Tilde{K_t} - \Tilde{L_t}  \right)
\end{equation}

\begin{equation}\tag{$\Tilde{6}$}
    \Tilde{Y}_t = \alpha \Tilde{K}_t + (1 - \alpha)(\Tilde{A}_t + \Tilde{L}_t)
\end{equation}

\begin{equation}
    Z_t = \left( \frac{W_t}{b} \right)^{ - \frac{1}{\chi}} \cdot C_t^{\frac{\theta}{\chi}}
\end{equation}

\begin{equation}
    Z_t 1  - L_t
\end{equation}

\begin{equation}
    \Tilde{Z}_t = - \frac{1}{\chi}\Tilde{W}_t + \frac{\theta}{\chi} \cdot \Tilde{C}_t
\end{equation}

\begin{equation}\tag{$\Tilde{2}$}
    \Tilde{L}_t = e_2 \Tilde{W}_t - e_3 \Tilde{C}_t
\end{equation}

$$
e_2 = \frac{1 - L^*}{L^*} \cdot \frac{1}{\chi} > 0
$$

$$
e_3 = \theta e_2 > 0
$$

\begin{equation}\tag{$\Tilde{4}$}
    \Tilde{R}_t = e_4 \left( \Tilde{A}_t + \Tilde{L}_t - \Tilde{K}_t  \right)
\end{equation}

$$
e_4 = \frac{\rho - \delta}{\rho}(1- \alpha) > 0
$$

\begin{equation}\tag{$\Tilde{5}$}
    \Tilde{K}_{t+1} = (1 - \delta) \Tilde{K}_t 0 e_5 \Tilde{Y}_t - e_6 \Tilde{C}_t - e_7 \Tilde{G_t}
\end{equation}

$$
e_5 = \frac{Y^*}{K^*}> 0
$$
Average product of capital, which is positive at the steady state.


$$
e_6 = e_5 \cdot \frac{C^*}{Y^*} > 0
$$

The ratio of consumption to output, or consumption divided by capital.


$$
e_7 = e_5 \cdot \frac{G^*_t}{Y^*} > 0
$$

\subsubsection*{Solving the dynamic model}


$$
E_t \Tilde{K}_{t +1} = \Tilde{K}_{t + 1}
$$

$$
E_t \Tilde{A}_{t + 1}= 
$$
\begin{equation}\label{matrix_solution}
\begingroup % keep the change local
\renewcommand*{\arraystretch}{2}
\begin{bmatrix}
E_t \Tilde{C}_{t +1} \\
\Tilde{K}_{t +1} 
\end{bmatrix}
=
\begin{bmatrix}
a_{1,1} & a_{1,2} \\
a_{2,1} & a_{2,2} 
\end{bmatrix}
\begin{bmatrix}
\Tilde{C}_t \\
\Tilde{K}_{t} 
\end{bmatrix}
+
\begin{bmatrix}
b_{1,1} & b_{1,2} \\
b_{2,1} & b_{2,2} 
\end{bmatrix}
\begin{bmatrix}
\Tilde{A}_t \\
\Tilde{G}_{t} 
\end{bmatrix}
\endgroup
\end{equation}


Fill in eigenvalues Candidate Solution


Laws of motion


$$
\tilde { c } _ { t } = a _ { CK} \cdot \tilde { k } _ { t } + a_ { CA } \cdot \tilde { A } _ { t } + a _ { CG } \cdot \tilde { G } _ { t }
$$

$$
\Tilde{K}_{t + 1} = b_{KK} \cdot \Tilde{K}_t + b_{KA} \cdot \Tilde{A}_t + b_{KG} \cdot \Tilde{G}_t
$$

From \ref{matrix_solution} we have:

$$
E_t \Tilde{C}_{t +1} = a_{CK} \cdot \Tilde{K}_{t + 1} + a_{CA} \cdot E_t \Tilde{A}_{t + 1} + a_{CG} \cdot E_t \Tilde{G}_{t + 1}
$$


$$
b _ { K G  } = a _ { 21 } \cdot a _ { CG } + b _ { 22 }
$$

$$
b _ { KA } = a _ { 2 1 } \cdot a _ { C A } + b _ { 21 }
$$


$$
b _ { KK } = a _ { 21 } a _ { CK } + a _ { 22 }
$$




\subsection{Empirical Validation}

\subsubsection{Calibration}

\subsection{Comparing the RBC model with data}

\paragraph{Pros}
\begin{enumerate}[(a)]
    \item Consumption is less volatile than output
    \item Investment is volatile than output ???
    \item Capital stock is much less volatile than output
    \item Real wages and the average product of labour are procyclical, as expected
    \item Employment is procyclical
    \item Time series created by the model is similar to data
\end{enumerate}

\paragraph{Cons}
\begin{enumerate}[(a)]
    \item Average product of labour is more procyclical than what is shown by data
    \item A positive correlation between employment and APL, but in reality the correlation is negative. 
    \item 

\end{enumerate}